iris/ProofIalloc.v
@@ -1156,7 +1156,7 @@ Section IallocClaim.
     procs_inv γs -∗
     dev_inv γu γd -∗
     disk_geom γd pd pav pu -∗
-    is_lock γk d_lock "virtio_disk"%string <{ disk_res γd pd pav pu }> -∗
+    is_lock γk d_lock "virtio_disk"%string (disk_res_at γd pd pav pu) -∗
     is_itable2 gtl cn γfs γi cov logstart nib dev -∗
     itable_inv -∗
     ic_escrows cn γfs γi cov logstart -∗
@@ -2026,7 +2026,7 @@ Section IallocScan.
     procs_inv γs -∗
     dev_inv γu γd -∗
     disk_geom γd pd pav pu -∗
-    is_lock γk d_lock "virtio_disk"%string <{ disk_res γd pd pav pu }> -∗
+    is_lock γk d_lock "virtio_disk"%string (disk_res_at γd pd pav pu) -∗
     is_itable2 gtl cn γfs γi cov logstart nib dev -∗
     itable_inv -∗
     ic_escrows cn γfs γi cov logstart -∗
