iris/ProofSysUnlink.v
@@ -712,7 +712,7 @@ Section ProofSysUnlinkBody.
     gen_cert -∗
     dev_inv gu gd -∗
     disk_geom gd pd pav pu -∗
-    is_lock gk d_lock "virtio_disk"%string <{ disk_res gd pd pav pu }> -∗
+    is_lock gk d_lock "virtio_disk"%string (disk_res_at gd pd pav pu) -∗
     bslots 3 -∗
     is_itable2 gtl cn gfs gi cov logstart nib dev -∗
     itable_inv -∗
@@ -1498,7 +1498,7 @@ Section ProofSysUnlinkBody.
     procs_inv gs -∗
     dev_inv gu gd -∗
     disk_geom gd pd pav pu -∗
-    is_lock gk d_lock "virtio_disk"%string <{ disk_res gd pd pav pu }> -∗
+    is_lock gk d_lock "virtio_disk"%string (disk_res_at gd pd pav pu) -∗
     bslots 3 -∗
     iref_slots 1 -∗
     log_op g u -∗
@@ -1654,7 +1654,7 @@ Section ProofSysUnlinkBody.
     gen_cert -∗
     dev_inv gu gd -∗
     disk_geom gd pd pav pu -∗
-    is_lock gk d_lock "virtio_disk"%string <{ disk_res gd pd pav pu }> -∗
+    is_lock gk d_lock "virtio_disk"%string (disk_res_at gd pd pav pu) -∗
     bslots 3 -∗
     is_itable2 gtl cn gfs gi cov logstart nib dev -∗
     itable_inv -∗
@@ -2708,7 +2708,7 @@ Section ProofSysUnlinkBody.
     procs_inv gs -∗
     dev_inv gu gd -∗
     disk_geom gd pd pav pu -∗
-    is_lock gk d_lock "virtio_disk"%string <{ disk_res gd pd pav pu }> -∗
+    is_lock gk d_lock "virtio_disk"%string (disk_res_at gd pd pav pu) -∗
     i_dev (ientry ki) ↦₄{DfracOwn (1/2)} dev -∗
     inode_meta (ientry ki) dni -∗
     inode_map gfs (ientry ki) bmi -∗
@@ -3260,7 +3260,7 @@ Section ProofSysUnlinkBody.
     procs_inv gs -∗
     dev_inv gu gd -∗
     disk_geom gd pd pav pu -∗
-    is_lock gk d_lock "virtio_disk"%string <{ disk_res gd pd pav pu }> -∗
+    is_lock gk d_lock "virtio_disk"%string (disk_res_at gd pd pav pu) -∗
     i_dev (ientry ki) ↦₄{DfracOwn (1/2)} dev -∗
     inode_meta (ientry ki) dni -∗
     inode_map gfs (ientry ki) bmi -∗
@@ -3512,7 +3512,7 @@ Section ProofSysUnlinkBody.
     gen_cert -∗
     dev_inv gu gd -∗
     disk_geom gd pd pav pu -∗
-    is_lock gk d_lock "virtio_disk"%string <{ disk_res gd pd pav pu }> -∗
+    is_lock gk d_lock "virtio_disk"%string (disk_res_at gd pd pav pu) -∗
     bslots 3 -∗
     is_itable2 gtl cn gfs gi cov logstart nib dev -∗
     itable_inv -∗
@@ -4282,7 +4282,7 @@ Section ProofSysUnlinkBody.
     gen_cert -∗
     dev_inv gu gd -∗
     disk_geom gd pd pav pu -∗
-    is_lock gk d_lock "virtio_disk"%string <{ disk_res gd pd pav pu }> -∗
+    is_lock gk d_lock "virtio_disk"%string (disk_res_at gd pd pav pu) -∗
     bslots 3 -∗
     is_itable2 gtl cn gfs gi cov logstart nib dev -∗
     itable_inv -∗
@@ -5831,7 +5831,7 @@ Section ProofSysUnlinkBody.
     gen_cert -∗
     dev_inv gu gd -∗
     disk_geom gd pd pav pu -∗
-    is_lock gk d_lock "virtio_disk"%string <{ disk_res gd pd pav pu }> -∗
+    is_lock gk d_lock "virtio_disk"%string (disk_res_at gd pd pav pu) -∗
     bslots 3 -∗
     is_itable2 gtl cn gfs gi cov logstart nib dev -∗
     itable_inv -∗
