iris/ProofSysUnlinkTails.v
@@ -566,7 +566,7 @@ Section ProofSysUnlinkTails.
     procs_inv gs -∗
     dev_inv gu gd -∗
     disk_geom gd pd pav pu -∗
-    is_lock gk d_lock "virtio_disk"%string <{ disk_res gd pd pav pu }> -∗
+    is_lock gk d_lock "virtio_disk"%string (disk_res_at gd pd pav pu) -∗
     log_op g u -∗
     (pa_stk sp0 1) ↦₈[KT1] (m !!! Regidx Rra : mword 64) -∗
     (pa_stk sp0 2) ↦₈[KT1] (m !!! Regidx Rs0 : mword 64) -∗
@@ -835,7 +835,7 @@ Section ProofSysUnlinkTails.
     procs_inv gs -∗
     dev_inv gu gd -∗
     disk_geom gd pd pav pu -∗
-    is_lock gk d_lock "virtio_disk"%string <{ disk_res gd pd pav pu }> -∗
+    is_lock gk d_lock "virtio_disk"%string (disk_res_at gd pd pav pu) -∗
     bslots 3 -∗
     log_op g u -∗
     (pa_stk sp0 1) ↦₈[KT1] (m !!! Regidx Rra : mword 64) -∗
@@ -1168,7 +1168,7 @@ Section ProofSysUnlinkTails.
     procs_inv gs -∗
     dev_inv gu gd -∗
     disk_geom gd pd pav pu -∗
-    is_lock gk d_lock "virtio_disk"%string <{ disk_res gd pd pav pu }> -∗
+    is_lock gk d_lock "virtio_disk"%string (disk_res_at gd pd pav pu) -∗
     bslots 3 -∗
     log_op g u -∗
     (pa_stk sp0 1) ↦₈[KT1] (m !!! Regidx Rra : mword 64) -∗
@@ -1375,7 +1375,7 @@ Section ProofSysUnlinkTails.
     procs_inv gs -∗
     dev_inv gu gd -∗
     disk_geom gd pd pav pu -∗
-    is_lock gk d_lock "virtio_disk"%string <{ disk_res gd pd pav pu }> -∗
+    is_lock gk d_lock "virtio_disk"%string (disk_res_at gd pd pav pu) -∗
     bslots 3 -∗
     log_op g u -∗
     (pa_stk sp0 1) ↦₈[KT1] (m !!! Regidx Rra : mword 64) -∗
